staged/Automation.v
@@ -7,6 +7,11 @@ Ltac funfold_hyp H env f :=
 Ltac funfold_ env f :=
   rewrites (>> norm_unk env f); [ unfold env; resolve_fn_in_env | ].
 
+Global Hint Rewrite norm_exists norm_forall norm_reassoc : norm_db.
+
+Ltac norm :=
+  autorewrite with norm_db.
+
 Tactic Notation "funfold" constr(env) constr(f) := funfold_ env f.
 Tactic Notation "funfold" constr(env) constr(f) "in" constr(H) := funfold_hyp H env f.
 
@@ -23,7 +28,7 @@ Ltac ent_step :=
     rewrite ent_seq_ex_reassoc
   | |- entails_under _ (ens_ \[_];; _) _ =>
     let H := fresh "H" in
-    simple apply ent_seq_ens_l; intros H
+    simple apply ent_seq_ens_l; intros H; destr H
 
   (* if there is an IH, try to use it *)
   | IH: context[entails_under ?env (unk _ _ _) _] |-
@@ -46,23 +51,25 @@ Ltac ent_step :=
   | |- entails_under _ _ (fex (fun _ => _)) =>
     simple apply ent_ex_r; eexists
   | |- entails_under _ (ens_ \[_]) (ens_ \[_]) =>
-    simple apply ent_ens_single; subst; intuition
+    simple apply ent_ens_single_pure; subst; intuition
+  | |- entails_under _ (ens_ _) (ens_ _) =>
+    simple apply ent_ens_single; xsimpl; subst; intuition
 
-    (* if all else fails, try basic tactics to hopefully get other steps to apply *)
-    | H: _ /\ _ |- _ =>
-      destruct H
-    | _: ?v = ?w |- _ =>
-      first [subst v | subst w]
+  (* if all else fails, try basic tactics to hopefully get other steps to apply *)
+  | H: _ /\ _ |- _ =>
+    destruct H
+  | _: ?v = ?w |- _ =>
+    first [subst v | subst w]
 
-    (* after we've tried everything, try to solve *)
-    | |- _ = _ =>
-      solve [simpl; simple apply eq_refl]
-      (* https://coq.inria.fr/doc/master/refman/proofs/writing-proofs/proof-mode.html#coq:flag.Solve-Unification-Constraints *)
-      (* solve [solve_constraints; reflexivity] *)
+  (* after we've tried everything, try to solve *)
+  | |- _ = _ =>
+    solve [simpl; simple apply eq_refl]
+    (* https://coq.inria.fr/doc/master/refman/proofs/writing-proofs/proof-mode.html#coq:flag.Solve-Unification-Constraints *)
+    (* solve [solve_constraints; reflexivity] *)
 
-    (* always have a no-match so we can repeat this *)
-    | |- ?g => idtac "no match"; idtac g; fail
-    end.
+  (* always have a no-match so we can repeat this *)
+  | |- ?g => idtac "no match"; idtac g; fail
+  end.
 
   Ltac solve_entailment :=
     repeat ent_step.
